simulate: better expression for the functional version of ADD

CoqOfRust/revm/revm_interpreter/gas/simulate/constants.v
@@ -3,10 +3,13 @@ Require Import CoqOfRust.links.M.
 Require Import CoqOfRust.simulate.M.
 Require Import revm.revm_interpreter.gas.links.constants.
 
+Definition VERYLOW : U64.t :=
+  {| Integer.value := 3 |}.
+
 Lemma VERYLOW_eq {Stack : Stack.t} (stack : Stack.to_Set Stack) :
   {{
     StackM.eval_f (Stack := Stack) run_VERYLOW stack 🌲
-    (Output.Success (Ref.immediate _ {| Integer.value := 3 |}), stack)
+    (Output.Success (Ref.immediate _ VERYLOW), stack)
   }}.
 Proof.
   cbn.
