CoqOfRust/revm/revm_interpreter/instructions/stack.v
@@ -225,7 +225,45 @@ Module instructions.
                                 [],
                               γ1_0
                             |) in
-                          Value.Tuple []))
+                          Value.Tuple []));
+                      fun γ =>
+                        ltac:(M.monadic
+                          (M.read (|
+                            let~ _ : Ty.tuple [] :=
+                              M.call_closure (|
+                                Ty.tuple [],
+                                M.get_trait_method (|
+                                  "revm_interpreter::interpreter_types::LoopControl",
+                                  Ty.associated_in_trait
+                                    "revm_interpreter::interpreter_types::InterpreterTypes"
+                                    []
+                                    []
+                                    WIRE
+                                    "Control",
+                                  [],
+                                  [],
+                                  "set_instruction_result",
+                                  [],
+                                  []
+                                |),
+                                [
+                                  M.borrow (|
+                                    Pointer.Kind.MutRef,
+                                    M.SubPointer.get_struct_record_field (|
+                                      M.deref (| M.read (| interpreter |) |),
+                                      "revm_interpreter::interpreter::Interpreter",
+                                      "control"
+                                    |)
+                                  |);
+                                  Value.StructTuple
+                                    "revm_interpreter::instruction_result::InstructionResult::StackUnderflow"
+                                    []
+                                    []
+                                    []
+                                ]
+                              |) in
+                            M.return_ (| Value.Tuple [] |)
+                          |)))
                     ]
                   |)
                 |)
@@ -1036,6 +1074,44 @@ Module instructions.
                                 ]
                               |) in
                             M.alloc (| Ty.tuple [], Value.Tuple [] |)
+                          |)));
+                      fun γ =>
+                        ltac:(M.monadic
+                          (M.read (|
+                            let~ _ : Ty.tuple [] :=
+                              M.call_closure (|
+                                Ty.tuple [],
+                                M.get_trait_method (|
+                                  "revm_interpreter::interpreter_types::LoopControl",
+                                  Ty.associated_in_trait
+                                    "revm_interpreter::interpreter_types::InterpreterTypes"
+                                    []
+                                    []
+                                    WIRE
+                                    "Control",
+                                  [],
+                                  [],
+                                  "set_instruction_result",
+                                  [],
+                                  []
+                                |),
+                                [
+                                  M.borrow (|
+                                    Pointer.Kind.MutRef,
+                                    M.SubPointer.get_struct_record_field (|
+                                      M.deref (| M.read (| interpreter |) |),
+                                      "revm_interpreter::interpreter::Interpreter",
+                                      "control"
+                                    |)
+                                  |);
+                                  Value.StructTuple
+                                    "revm_interpreter::instruction_result::InstructionResult::StackUnderflow"
+                                    []
+                                    []
+                                    []
+                                ]
+                              |) in
+                            M.return_ (| Value.Tuple [] |)
                           |)))
                     ]
                   |)
