CoqOfRust/revm/revm_interpreter/simulate/interpreter_types.v
@@ -3,6 +3,7 @@ Require Import CoqOfRust.links.M.
 Require Import CoqOfRust.simulate.M.
 Require Import alloy_primitives.links.aliases.
 Require Import revm.revm_interpreter.links.gas.
+Require Import revm.revm_interpreter.links.instruction_result.
 Require Import revm.revm_interpreter.links.interpreter.
 Require Import revm.revm_interpreter.links.interpreter_types.
 
@@ -10,6 +11,13 @@ Module Loop.
  Class C
       (WIRE_types : InterpreterTypes.Types.t) `{InterpreterTypes.Types.AreLinks WIRE_types} :
       Set := {
+    (* fn set_instruction_result(&mut self, result: InstructionResult); *)
+    set_instruction_result :
+      forall
+        (self : WIRE_types.(InterpreterTypes.Types.Control))
+        (result : InstructionResult.t),
+      WIRE_types.(InterpreterTypes.Types.Control);
+    (* fn gas(&mut self) -> &mut Gas; *)
     gas : RefStub.t WIRE_types.(InterpreterTypes.Types.Control) Gas.t;
   }.
 
@@ -20,10 +28,35 @@ Module Loop.
         (run_InterpreterTypes_for_WIRE : InterpreterTypes.Run WIRE WIRE_types)
         (I : C WIRE_types) :
         Prop := {
-      gas
-          (Stack : list Set)
+      set_instruction_result
+          (StackRest : list Set)
           (interpreter : Interpreter.t WIRE WIRE_types)
-          (stack_rest : Stack.to_Set Stack) :
+          (stack_rest : Stack.to_Set StackRest)
+          (result : InstructionResult.t) :
+        let ref_interpreter : Ref.t Pointer.Kind.MutRef _ := make_ref 0 in
+        let ref_self := {| Ref.core :=
+            SubPointer.Runner.apply
+              ref_interpreter.(Ref.core)
+              Interpreter.SubPointer.get_control
+        |} in
+        let control' :=
+          I.(set_instruction_result) interpreter.(Interpreter.control) result in
+        {{
+          StackM.eval_f (Stack := Interpreter.t WIRE WIRE_types :: StackRest)
+            (run_InterpreterTypes_for_WIRE.(InterpreterTypes.run_LoopControl_for_Control).(LoopControl.set_instruction_result).(TraitMethod.run)
+              ref_self
+              result
+            )
+            (interpreter, stack_rest) 🌲
+          (
+            Output.Success tt,
+            (interpreter <| Interpreter.control := control' |>, stack_rest)
+          )
+        }};
+      gas
+          (StackRest : list Set)
+          (interpreter : Interpreter.t WIRE WIRE_types)
+          (stack_rest : Stack.to_Set StackRest) :
         let ref_interpreter : Ref.t Pointer.Kind.MutRef _ := make_ref 0 in
         let ref_self := {| Ref.core :=
             SubPointer.Runner.apply
@@ -31,7 +64,7 @@ Module Loop.
               Interpreter.SubPointer.get_control
         |} in
         {{
-          StackM.eval_f (Stack := Interpreter.t WIRE WIRE_types :: Stack)
+          StackM.eval_f (Stack := Interpreter.t WIRE WIRE_types :: StackRest)
             (run_InterpreterTypes_for_WIRE.(InterpreterTypes.run_LoopControl_for_Control).(LoopControl.gas).(TraitMethod.run)
               ref_self
             )
@@ -68,6 +101,7 @@ Module Stack.
   Class C
       (WIRE_types : InterpreterTypes.Types.t) `{InterpreterTypes.Types.AreLinks WIRE_types} :
       Type := {
+    (* fn popn_top<const POPN: usize>(&mut self) -> Option<([U256; POPN], &mut U256)>; *)
     popn_top :
       forall
         (POPN : Usize.t)
