CoqOfRust/ruint/simulate/add.v
@@ -1,0 +1,14 @@
+Require Import CoqOfRust.CoqOfRust.
+Require Import CoqOfRust.links.M.
+Require Import ruint.links.add.
+
+Module Impl_Uint.
+  Parameter wrapping_add :
+    forall {BITS LIMBS : Usize.t} (x1 x2 : lib.Uint.t BITS LIMBS),
+    lib.Uint.t BITS LIMBS.
+
+  Lemma wrapping_add_eq (BITS LIMBS : Usize.t) (x1 x2 : lib.Uint.t BITS LIMBS) :
+    links.M.evaluate (add.Impl_Uint.run_wrapping_add BITS LIMBS x1 x2).(Run.run_f) =
+    links.M.LowM.Pure (Output.Success (wrapping_add x1 x2)).
+  Admitted.
+End Impl_Uint.
