CoqOfRust/revm/revm_bytecode/eof/printer.v
@@ -1160,6 +1160,323 @@ Module eof.
                                             |)
                                           |) in
                                         M.alloc (| Ty.tuple [], Value.Tuple [] |)
+                                      |)));
+                                  fun γ =>
+                                    ltac:(M.monadic
+                                      (M.read (|
+                                        let~ _ : Ty.tuple [] :=
+                                          M.read (|
+                                            let~ _ : Ty.tuple [] :=
+                                              M.call_closure (|
+                                                Ty.tuple [],
+                                                M.get_function (|
+                                                  "std::io::stdio::_print",
+                                                  [],
+                                                  []
+                                                |),
+                                                [
+                                                  M.call_closure (|
+                                                    Ty.path "core::fmt::Arguments",
+                                                    M.get_associated_function (|
+                                                      Ty.path "core::fmt::Arguments",
+                                                      "new_v1_formatted",
+                                                      [],
+                                                      []
+                                                    |),
+                                                    [
+                                                      M.call_closure (|
+                                                        Ty.apply
+                                                          (Ty.path "&")
+                                                          []
+                                                          [
+                                                            Ty.apply
+                                                              (Ty.path "slice")
+                                                              []
+                                                              [
+                                                                Ty.apply
+                                                                  (Ty.path "&")
+                                                                  []
+                                                                  [ Ty.path "str" ]
+                                                              ]
+                                                          ],
+                                                        M.pointer_coercion
+                                                          M.PointerCoercion.Unsize
+                                                          (Ty.apply
+                                                            (Ty.path "&")
+                                                            []
+                                                            [
+                                                              Ty.apply
+                                                                (Ty.path "array")
+                                                                [ Value.Integer IntegerKind.Usize 2
+                                                                ]
+                                                                [
+                                                                  Ty.apply
+                                                                    (Ty.path "&")
+                                                                    []
+                                                                    [ Ty.path "str" ]
+                                                                ]
+                                                            ])
+                                                          (Ty.apply
+                                                            (Ty.path "&")
+                                                            []
+                                                            [
+                                                              Ty.apply
+                                                                (Ty.path "slice")
+                                                                []
+                                                                [
+                                                                  Ty.apply
+                                                                    (Ty.path "&")
+                                                                    []
+                                                                    [ Ty.path "str" ]
+                                                                ]
+                                                            ]),
+                                                        [
+                                                          M.borrow (|
+                                                            Pointer.Kind.Ref,
+                                                            M.deref (|
+                                                              M.borrow (|
+                                                                Pointer.Kind.Ref,
+                                                                M.alloc (|
+                                                                  Ty.apply
+                                                                    (Ty.path "array")
+                                                                    [
+                                                                      Value.Integer
+                                                                        IntegerKind.Usize
+                                                                        2
+                                                                    ]
+                                                                    [
+                                                                      Ty.apply
+                                                                        (Ty.path "&")
+                                                                        []
+                                                                        [ Ty.path "str" ]
+                                                                    ],
+                                                                  Value.Array
+                                                                    [
+                                                                      mk_str (|
+                                                                        "Unknown opcode: 0x"
+                                                                      |);
+                                                                      mk_str (| "
+" |)
+                                                                    ]
+                                                                |)
+                                                              |)
+                                                            |)
+                                                          |)
+                                                        ]
+                                                      |);
+                                                      M.call_closure (|
+                                                        Ty.apply
+                                                          (Ty.path "&")
+                                                          []
+                                                          [
+                                                            Ty.apply
+                                                              (Ty.path "slice")
+                                                              []
+                                                              [ Ty.path "core::fmt::rt::Argument" ]
+                                                          ],
+                                                        M.pointer_coercion
+                                                          M.PointerCoercion.Unsize
+                                                          (Ty.apply
+                                                            (Ty.path "&")
+                                                            []
+                                                            [
+                                                              Ty.apply
+                                                                (Ty.path "array")
+                                                                [ Value.Integer IntegerKind.Usize 1
+                                                                ]
+                                                                [ Ty.path "core::fmt::rt::Argument"
+                                                                ]
+                                                            ])
+                                                          (Ty.apply
+                                                            (Ty.path "&")
+                                                            []
+                                                            [
+                                                              Ty.apply
+                                                                (Ty.path "slice")
+                                                                []
+                                                                [ Ty.path "core::fmt::rt::Argument"
+                                                                ]
+                                                            ]),
+                                                        [
+                                                          M.borrow (|
+                                                            Pointer.Kind.Ref,
+                                                            M.deref (|
+                                                              M.borrow (|
+                                                                Pointer.Kind.Ref,
+                                                                M.alloc (|
+                                                                  Ty.apply
+                                                                    (Ty.path "array")
+                                                                    [
+                                                                      Value.Integer
+                                                                        IntegerKind.Usize
+                                                                        1
+                                                                    ]
+                                                                    [
+                                                                      Ty.path
+                                                                        "core::fmt::rt::Argument"
+                                                                    ],
+                                                                  Value.Array
+                                                                    [
+                                                                      M.call_closure (|
+                                                                        Ty.path
+                                                                          "core::fmt::rt::Argument",
+                                                                        M.get_associated_function (|
+                                                                          Ty.path
+                                                                            "core::fmt::rt::Argument",
+                                                                          "new_upper_hex",
+                                                                          [],
+                                                                          [ Ty.path "u8" ]
+                                                                        |),
+                                                                        [
+                                                                          M.borrow (|
+                                                                            Pointer.Kind.Ref,
+                                                                            M.deref (|
+                                                                              M.borrow (|
+                                                                                Pointer.Kind.Ref,
+                                                                                op
+                                                                              |)
+                                                                            |)
+                                                                          |)
+                                                                        ]
+                                                                      |)
+                                                                    ]
+                                                                |)
+                                                              |)
+                                                            |)
+                                                          |)
+                                                        ]
+                                                      |);
+                                                      M.call_closure (|
+                                                        Ty.apply
+                                                          (Ty.path "&")
+                                                          []
+                                                          [
+                                                            Ty.apply
+                                                              (Ty.path "slice")
+                                                              []
+                                                              [ Ty.path "core::fmt::rt::Placeholder"
+                                                              ]
+                                                          ],
+                                                        M.pointer_coercion
+                                                          M.PointerCoercion.Unsize
+                                                          (Ty.apply
+                                                            (Ty.path "&")
+                                                            []
+                                                            [
+                                                              Ty.apply
+                                                                (Ty.path "array")
+                                                                [ Value.Integer IntegerKind.Usize 1
+                                                                ]
+                                                                [
+                                                                  Ty.path
+                                                                    "core::fmt::rt::Placeholder"
+                                                                ]
+                                                            ])
+                                                          (Ty.apply
+                                                            (Ty.path "&")
+                                                            []
+                                                            [
+                                                              Ty.apply
+                                                                (Ty.path "slice")
+                                                                []
+                                                                [
+                                                                  Ty.path
+                                                                    "core::fmt::rt::Placeholder"
+                                                                ]
+                                                            ]),
+                                                        [
+                                                          M.borrow (|
+                                                            Pointer.Kind.Ref,
+                                                            M.deref (|
+                                                              M.borrow (|
+                                                                Pointer.Kind.Ref,
+                                                                M.alloc (|
+                                                                  Ty.apply
+                                                                    (Ty.path "array")
+                                                                    [
+                                                                      Value.Integer
+                                                                        IntegerKind.Usize
+                                                                        1
+                                                                    ]
+                                                                    [
+                                                                      Ty.path
+                                                                        "core::fmt::rt::Placeholder"
+                                                                    ],
+                                                                  Value.Array
+                                                                    [
+                                                                      M.call_closure (|
+                                                                        Ty.path
+                                                                          "core::fmt::rt::Placeholder",
+                                                                        M.get_associated_function (|
+                                                                          Ty.path
+                                                                            "core::fmt::rt::Placeholder",
+                                                                          "new",
+                                                                          [],
+                                                                          []
+                                                                        |),
+                                                                        [
+                                                                          Value.Integer
+                                                                            IntegerKind.Usize
+                                                                            0;
+                                                                          Value.UnicodeChar 32;
+                                                                          Value.StructTuple
+                                                                            "core::fmt::rt::Alignment::Unknown"
+                                                                            []
+                                                                            []
+                                                                            [];
+                                                                          Value.Integer
+                                                                            IntegerKind.U32
+                                                                            8;
+                                                                          Value.StructTuple
+                                                                            "core::fmt::rt::Count::Implied"
+                                                                            []
+                                                                            []
+                                                                            [];
+                                                                          Value.StructTuple
+                                                                            "core::fmt::rt::Count::Is"
+                                                                            []
+                                                                            []
+                                                                            [
+                                                                              Value.Integer
+                                                                                IntegerKind.Usize
+                                                                                2
+                                                                            ]
+                                                                        ]
+                                                                      |)
+                                                                    ]
+                                                                |)
+                                                              |)
+                                                            |)
+                                                          |)
+                                                        ]
+                                                      |);
+                                                      M.call_closure (|
+                                                        Ty.path "core::fmt::rt::UnsafeArg",
+                                                        M.get_associated_function (|
+                                                          Ty.path "core::fmt::rt::UnsafeArg",
+                                                          "new",
+                                                          [],
+                                                          []
+                                                        |),
+                                                        []
+                                                      |)
+                                                    ]
+                                                  |)
+                                                ]
+                                              |) in
+                                            M.alloc (| Ty.tuple [], Value.Tuple [] |)
+                                          |) in
+                                        let~ _ : Ty.tuple [] :=
+                                          let β := i in
+                                          M.write (|
+                                            β,
+                                            M.call_closure (|
+                                              Ty.path "usize",
+                                              BinOp.Wrap.add,
+                                              [ M.read (| β |); Value.Integer IntegerKind.Usize 1 ]
+                                            |)
+                                          |) in
+                                        M.continue (||)
                                       |)))
                                 ]
                               |)
