CoqOfRust/revm/revm_interpreter/instructions/control.v
@@ -727,6 +727,44 @@ Module instructions.
                                 ]
                               |) in
                             M.alloc (| Ty.tuple [], Value.Tuple [] |)
+                          |)));
+                      fun γ =>
+                        ltac:(M.monadic
+                          (M.read (|
+                            let~ _ : Ty.tuple [] :=
+                              M.call_closure (|
+                                Ty.tuple [],
+                                M.get_trait_method (|
+                                  "revm_interpreter::interpreter_types::LoopControl",
+                                  Ty.associated_in_trait
+                                    "revm_interpreter::interpreter_types::InterpreterTypes"
+                                    []
+                                    []
+                                    WIRE
+                                    "Control",
+                                  [],
+                                  [],
+                                  "set_instruction_result",
+                                  [],
+                                  []
+                                |),
+                                [
+                                  M.borrow (|
+                                    Pointer.Kind.MutRef,
+                                    M.SubPointer.get_struct_record_field (|
+                                      M.deref (| M.read (| interpreter |) |),
+                                      "revm_interpreter::interpreter::Interpreter",
+                                      "control"
+                                    |)
+                                  |);
+                                  Value.StructTuple
+                                    "revm_interpreter::instruction_result::InstructionResult::StackUnderflow"
+                                    []
+                                    []
+                                    []
+                                ]
+                              |) in
+                            M.return_ (| Value.Tuple [] |)
                           |)))
                     ]
                   |)
@@ -1420,6 +1458,44 @@ Module instructions.
                                 ]
                               |) in
                             M.alloc (| Ty.tuple [], Value.Tuple [] |)
+                          |)));
+                      fun γ =>
+                        ltac:(M.monadic
+                          (M.read (|
+                            let~ _ : Ty.tuple [] :=
+                              M.call_closure (|
+                                Ty.tuple [],
+                                M.get_trait_method (|
+                                  "revm_interpreter::interpreter_types::LoopControl",
+                                  Ty.associated_in_trait
+                                    "revm_interpreter::interpreter_types::InterpreterTypes"
+                                    []
+                                    []
+                                    WIRE
+                                    "Control",
+                                  [],
+                                  [],
+                                  "set_instruction_result",
+                                  [],
+                                  []
+                                |),
+                                [
+                                  M.borrow (|
+                                    Pointer.Kind.MutRef,
+                                    M.SubPointer.get_struct_record_field (|
+                                      M.deref (| M.read (| interpreter |) |),
+                                      "revm_interpreter::interpreter::Interpreter",
+                                      "control"
+                                    |)
+                                  |);
+                                  Value.StructTuple
+                                    "revm_interpreter::instruction_result::InstructionResult::StackUnderflow"
+                                    []
+                                    []
+                                    []
+                                ]
+                              |) in
+                            M.return_ (| Value.Tuple [] |)
                           |)))
                     ]
                   |)
@@ -1674,6 +1750,44 @@ Module instructions.
                                 ]
                               |) in
                             M.alloc (| Ty.tuple [], Value.Tuple [] |)
+                          |)));
+                      fun γ =>
+                        ltac:(M.monadic
+                          (M.read (|
+                            let~ _ : Ty.tuple [] :=
+                              M.call_closure (|
+                                Ty.tuple [],
+                                M.get_trait_method (|
+                                  "revm_interpreter::interpreter_types::LoopControl",
+                                  Ty.associated_in_trait
+                                    "revm_interpreter::interpreter_types::InterpreterTypes"
+                                    []
+                                    []
+                                    WIRE
+                                    "Control",
+                                  [],
+                                  [],
+                                  "set_instruction_result",
+                                  [],
+                                  []
+                                |),
+                                [
+                                  M.borrow (|
+                                    Pointer.Kind.MutRef,
+                                    M.SubPointer.get_struct_record_field (|
+                                      M.deref (| M.read (| interpreter |) |),
+                                      "revm_interpreter::interpreter::Interpreter",
+                                      "control"
+                                    |)
+                                  |);
+                                  Value.StructTuple
+                                    "revm_interpreter::instruction_result::InstructionResult::StackUnderflow"
+                                    []
+                                    []
+                                    []
+                                ]
+                              |) in
+                            M.return_ (| Value.Tuple [] |)
                           |)))
                     ]
                   |)
@@ -1980,6 +2094,44 @@ Module instructions.
                                   |)));
                               fun γ => ltac:(M.monadic (Value.Tuple []))
                             ]
+                          |)));
+                      fun γ =>
+                        ltac:(M.monadic
+                          (M.read (|
+                            let~ _ : Ty.tuple [] :=
+                              M.call_closure (|
+                                Ty.tuple [],
+                                M.get_trait_method (|
+                                  "revm_interpreter::interpreter_types::LoopControl",
+                                  Ty.associated_in_trait
+                                    "revm_interpreter::interpreter_types::InterpreterTypes"
+                                    []
+                                    []
+                                    WIRE
+                                    "Control",
+                                  [],
+                                  [],
+                                  "set_instruction_result",
+                                  [],
+                                  []
+                                |),
+                                [
+                                  M.borrow (|
+                                    Pointer.Kind.MutRef,
+                                    M.SubPointer.get_struct_record_field (|
+                                      M.deref (| M.read (| interpreter |) |),
+                                      "revm_interpreter::interpreter::Interpreter",
+                                      "control"
+                                    |)
+                                  |);
+                                  Value.StructTuple
+                                    "revm_interpreter::instruction_result::InstructionResult::StackUnderflow"
+                                    []
+                                    []
+                                    []
+                                ]
+                              |) in
+                            M.return_ (| Value.Tuple [] |)
                           |)))
                     ]
                   |)
@@ -3175,6 +3327,45 @@ Module instructions.
                                 ]
                               |) in
                             M.alloc (| Ty.tuple [], Value.Tuple [] |)
+                          |)));
+                      fun γ =>
+                        ltac:(M.monadic
+                          (M.call_closure (|
+                            Ty.path "never",
+                            M.get_function (| "core::panicking::panic_fmt", [], [] |),
+                            [
+                              M.call_closure (|
+                                Ty.path "core::fmt::Arguments",
+                                M.get_associated_function (|
+                                  Ty.path "core::fmt::Arguments",
+                                  "new_const",
+                                  [ Value.Integer IntegerKind.Usize 1 ],
+                                  []
+                                |),
+                                [
+                                  M.borrow (|
+                                    Pointer.Kind.Ref,
+                                    M.deref (|
+                                      M.borrow (|
+                                        Pointer.Kind.Ref,
+                                        M.alloc (|
+                                          Ty.apply
+                                            (Ty.path "array")
+                                            [ Value.Integer IntegerKind.Usize 1 ]
+                                            [ Ty.apply (Ty.path "&") [] [ Ty.path "str" ] ],
+                                          Value.Array
+                                            [
+                                              mk_str (|
+                                                "Invalid EOF in execution, expecting correct intermediate in callf"
+                                              |)
+                                            ]
+                                        |)
+                                      |)
+                                    |)
+                                  |)
+                                ]
+                              |)
+                            ]
                           |)))
                     ]
                   |)
@@ -3488,6 +3679,40 @@ Module instructions.
                                 ]
                               |) in
                             M.alloc (| Ty.tuple [], Value.Tuple [] |)
+                          |)));
+                      fun γ =>
+                        ltac:(M.monadic
+                          (M.call_closure (|
+                            Ty.path "never",
+                            M.get_function (| "core::panicking::panic_fmt", [], [] |),
+                            [
+                              M.call_closure (|
+                                Ty.path "core::fmt::Arguments",
+                                M.get_associated_function (|
+                                  Ty.path "core::fmt::Arguments",
+                                  "new_const",
+                                  [ Value.Integer IntegerKind.Usize 1 ],
+                                  []
+                                |),
+                                [
+                                  M.borrow (|
+                                    Pointer.Kind.Ref,
+                                    M.deref (|
+                                      M.borrow (|
+                                        Pointer.Kind.Ref,
+                                        M.alloc (|
+                                          Ty.apply
+                                            (Ty.path "array")
+                                            [ Value.Integer IntegerKind.Usize 1 ]
+                                            [ Ty.apply (Ty.path "&") [] [ Ty.path "str" ] ],
+                                          Value.Array [ mk_str (| "Expected function frame" |) ]
+                                        |)
+                                      |)
+                                    |)
+                                  |)
+                                ]
+                              |)
+                            ]
                           |)))
                     ]
                   |)
@@ -5380,6 +5605,44 @@ Module instructions.
                             ]
                           |) in
                         M.alloc (| Ty.tuple [], Value.Tuple [] |)
+                      |)));
+                  fun γ =>
+                    ltac:(M.monadic
+                      (M.read (|
+                        let~ _ : Ty.tuple [] :=
+                          M.call_closure (|
+                            Ty.tuple [],
+                            M.get_trait_method (|
+                              "revm_interpreter::interpreter_types::LoopControl",
+                              Ty.associated_in_trait
+                                "revm_interpreter::interpreter_types::InterpreterTypes"
+                                []
+                                []
+                                impl_InterpreterTypes
+                                "Control",
+                              [],
+                              [],
+                              "set_instruction_result",
+                              [],
+                              []
+                            |),
+                            [
+                              M.borrow (|
+                                Pointer.Kind.MutRef,
+                                M.SubPointer.get_struct_record_field (|
+                                  M.deref (| M.read (| interpreter |) |),
+                                  "revm_interpreter::interpreter::Interpreter",
+                                  "control"
+                                |)
+                              |);
+                              Value.StructTuple
+                                "revm_interpreter::instruction_result::InstructionResult::StackUnderflow"
+                                []
+                                []
+                                []
+                            ]
+                          |) in
+                        M.return_ (| Value.Tuple [] |)
                       |)))
                 ]
               |)))
